{
 "cells": [
  {
   "cell_type": "markdown",
   "id": "5e50c61d",
   "metadata": {},
   "source": [
    "# Problem 4: Optimal estimation\n",
    "\n",
    "We have two measurements\n",
    "$$\n",
    "Y_i = h_i X + \\epsilon_i,\\quad i=1,2,\n",
    "$$\n",
    "with \\(h_1=1,\\; h_2=2\\). The noise satisfies\n",
    "$$\n",
    "\\mathbb E[\\epsilon_i]=0,\\qquad \\mathbb E[\\epsilon_i^2]=\\sigma_i^2,\n",
    "$$\n",
    "and \\(\\epsilon_1,\\epsilon_2\\) are uncorrelated. Also \\( \\mathbb E[X\\epsilon_i]=0\\).\n",
    "\n",
    "We consider an estimator of the form\n",
    "$$\n",
    "\\hat X = a_1 Y_1 + a_2 Y_2,\n",
    "$$\n",
    "where \\(a_1,a_2\\) are constants independent of \\(X\\).\n",
    "\n",
    "---\n",
    "\n",
    "## (a)(i) Unbiasedness constraint\n",
    "\n",
    "First compute the expectation:\n",
    "$$\n",
    "\\mathbb E[Y_1]=\\mathbb E[X+\\epsilon_1]=X,\\qquad\n",
    "\\mathbb E[Y_2]=\\mathbb E[2X+\\epsilon_2]=2X.\n",
    "$$\n",
    "\n",
    "Thus\n",
    "$$\n",
    "\\mathbb E[\\hat X]=a_1 \\mathbb E[Y_1] + a_2 \\mathbb E[Y_2]\n",
    "= a_1 X + a_2 (2X) = (a_1+2a_2)X.\n",
    "$$\n",
    "\n",
    "For \\(\\hat X\\) to be unbiased, we require \\(\\mathbb E[\\hat X]=X\\) for all \\(X\\), hence\n",
    "$$\n",
    "\\boxed{a_1 + 2a_2 = 1.}\n",
    "$$\n",
    "\n",
    "---\n",
    "\n",
    "## (a)(ii) Minimize the MSE \\(\\mathbb E[(X-\\hat X)^2]\\)\n",
    "\n",
    "Write the estimation error:\n",
    "$$\n",
    "\\begin{aligned}\n",
    "X-\\hat X\n",
    "&= X - a_1(X+\\epsilon_1) - a_2(2X+\\epsilon_2) \\\\\n",
    "&= \\bigl(1-a_1-2a_2\\bigr)X - a_1\\epsilon_1 - a_2\\epsilon_2.\n",
    "\\end{aligned}\n",
    "$$\n",
    "\n",
    "Under the unbiasedness constraint \\(a_1+2a_2=1\\), the \\(X\\)-term vanishes:\n",
    "$$\n",
    "X-\\hat X = -a_1\\epsilon_1 - a_2\\epsilon_2.\n",
    "$$\n",
    "\n",
    "Therefore the mean-square error becomes\n",
    "$$\n",
    "\\begin{aligned}\n",
    "\\mathbb E[(X-\\hat X)^2]\n",
    "&= \\mathbb E\\bigl[(a_1\\epsilon_1 + a_2\\epsilon_2)^2\\bigr] \\\\\n",
    "&= a_1^2\\mathbb E[\\epsilon_1^2] + a_2^2\\mathbb E[\\epsilon_2^2]\n",
    "    + 2a_1a_2\\mathbb E[\\epsilon_1\\epsilon_2].\n",
    "\\end{aligned}\n",
    "$$\n",
    "\n",
    "Since \\(\\epsilon_1,\\epsilon_2\\) are uncorrelated, \\(\\mathbb E[\\epsilon_1\\epsilon_2]=0\\). Hence\n",
    "$$\n",
    "\\boxed{\\text{MSE}(a_1,a_2)=a_1^2\\sigma_1^2 + a_2^2\\sigma_2^2}\n",
    "\\quad \\text{subject to } a_1+2a_2=1.\n",
    "$$\n",
    "\n",
    "### Lagrange multiplier\n",
    "Minimize\n",
    "$$\n",
    "J(a_1,a_2,\\lambda)=a_1^2\\sigma_1^2+a_2^2\\sigma_2^2+\\lambda(a_1+2a_2-1).\n",
    "$$\n",
    "\n",
    "Set partial derivatives to zero:\n",
    "$$\n",
    "\\frac{\\partial J}{\\partial a_1}=2a_1\\sigma_1^2+\\lambda=0\n",
    "\\;\\Rightarrow\\;\n",
    "a_1=-\\frac{\\lambda}{2\\sigma_1^2},\n",
    "$$\n",
    "$$\n",
    "\\frac{\\partial J}{\\partial a_2}=2a_2\\sigma_2^2+2\\lambda=0\n",
    "\\;\\Rightarrow\\;\n",
    "a_2=-\\frac{\\lambda}{\\sigma_2^2}.\n",
    "$$\n",
    "\n",
    "Use the constraint \\(a_1+2a_2=1\\):\n",
    "$$\n",
    "-\\frac{\\lambda}{2\\sigma_1^2} + 2\\Bigl(-\\frac{\\lambda}{\\sigma_2^2}\\Bigr)=1\n",
    "\\;\\Rightarrow\\;\n",
    "-\\lambda\\Bigl(\\frac{1}{2\\sigma_1^2}+\\frac{2}{\\sigma_2^2}\\Bigr)=1.\n",
    "$$\n",
    "\n",
    "Thus\n",
    "$$\n",
    "\\lambda=-\\frac{1}{\\frac{1}{2\\sigma_1^2}+\\frac{2}{\\sigma_2^2}}.\n",
    "$$\n",
    "\n",
    "Plugging back gives\n",
    "$$\n",
    "a_1=\\frac{\\frac{1}{2\\sigma_1^2}}{\\frac{1}{2\\sigma_1^2}+\\frac{2}{\\sigma_2^2}}\n",
    "=\\boxed{\\frac{\\sigma_2^2}{\\sigma_2^2+4\\sigma_1^2}},\n",
    "$$\n",
    "$$\n",
    "a_2=\\frac{\\frac{1}{\\sigma_2^2}}{\\frac{1}{2\\sigma_1^2}+\\frac{2}{\\sigma_2^2}}\n",
    "=\\boxed{\\frac{2\\sigma_1^2}{\\sigma_2^2+4\\sigma_1^2}}.\n",
    "$$\n",
    "\n",
    "### Minimum MSE value\n",
    "$$\n",
    "\\begin{aligned}\n",
    "\\text{MSE}_{\\min}\n",
    "&= a_1^2\\sigma_1^2 + a_2^2\\sigma_2^2 \\\\\n",
    "&= \\frac{\\sigma_2^4}{(\\sigma_2^2+4\\sigma_1^2)^2}\\sigma_1^2\n",
    " + \\frac{4\\sigma_1^4}{(\\sigma_2^2+4\\sigma_1^2)^2}\\sigma_2^2 \\\\\n",
    "&= \\frac{\\sigma_1^2\\sigma_2^2(\\sigma_2^2+4\\sigma_1^2)}{(\\sigma_2^2+4\\sigma_1^2)^2}\n",
    "= \\boxed{\\frac{\\sigma_1^2\\sigma_2^2}{\\sigma_2^2+4\\sigma_1^2}}.\n",
    "\\end{aligned}\n",
    "$$\n",
    "\n",
    "---\n",
    "\n",
    "\n"
   ]
  }
 ],
 "metadata": {
  "language_info": {
   "name": "python"
  }
 },
 "nbformat": 4,
 "nbformat_minor": 5
}
