{
 "cells": [
  {
   "cell_type": "markdown",
   "id": "a6c89125",
   "metadata": {},
   "source": [
    "# ESE 650 HW1 — Problem 3(a)  \n",
    "## Forward–Backward Algorithm (Detailed Derivations)\n",
    "\n",
    "We consider a Hidden Markov Model (HMM) with\n",
    "\n",
    "- Hidden states: $X_k \\in \\{x_1, \\dots, x_N\\}$\n",
    "- Observations: $Y_k$\n",
    "- State transition matrix:\n",
    "  $$\n",
    "  T_{ij} = P(X_{k+1} = x_j \\mid X_k = x_i)\n",
    "  $$\n",
    "- Observation (emission) matrix:\n",
    "  $$\n",
    "  M_{i,y} = P(Y_k = y \\mid X_k = x_i)\n",
    "  $$\n",
    "\n",
    "The forward and backward variables are defined as\n",
    "$$\n",
    "\\alpha_k(x) = P(Y_{1:k}, X_k = x),\n",
    "$$\n",
    "$$\n",
    "\\beta_k(x) = P(Y_{k+1:t} \\mid X_k = x).\n",
    "$$\n",
    "\n",
    "Throughout the derivation, we use the following HMM assumptions:\n",
    "\n",
    "1. **Markov property**:\n",
    "   $$\n",
    "   P(X_{k+1} \\mid X_{1:k}, Y_{1:k}) = P(X_{k+1} \\mid X_k)\n",
    "   $$\n",
    "2. **Conditional independence of observations**:\n",
    "   $$\n",
    "   P(Y_k \\mid X_{1:t}, Y_{\\neq k}) = P(Y_k \\mid X_k)\n",
    "   $$\n",
    "\n",
    "Boundary cases $k \\in \\{1,t\\}$ are ignored.\n",
    "\n",
    "---\n",
    "\n",
    "## (1) Derive $P(X_{k+1} = x_j \\mid X_k = x_i, Y_{1:t})$\n",
    "\n",
    "### Step 1: Definition of conditional probability\n",
    "\n",
    "$$\n",
    "P(X_{k+1} = x_j \\mid X_k = x_i, Y_{1:t})\n",
    "=\n",
    "\\frac{\n",
    "P(X_{k+1} = x_j, X_k = x_i, Y_{1:t})\n",
    "}{\n",
    "P(X_k = x_i, Y_{1:t})\n",
    "}\n",
    "$$\n",
    "\n",
    "---\n",
    "\n",
    "### Step 2: Compute the numerator\n",
    "\n",
    "Split the observation sequence into past and future:\n",
    "$$\n",
    "Y_{1:t} = (Y_{1:k}, Y_{k+1:t})\n",
    "$$\n",
    "\n",
    "Then\n",
    "$$\n",
    "P(X_{k+1} = x_j, X_k = x_i, Y_{1:t})\n",
    "=\n",
    "P(Y_{1:k}, X_k = x_i)\\,\n",
    "P(X_{k+1} = x_j, Y_{k+1:t} \\mid X_k = x_i)\n",
    "$$\n",
    "\n",
    "By the Markov property,\n",
    "$$\n",
    "P(X_{k+1} = x_j, Y_{k+1:t} \\mid X_k = x_i)\n",
    "=\n",
    "P(X_{k+1} = x_j \\mid X_k = x_i)\\,\n",
    "P(Y_{k+1:t} \\mid X_{k+1} = x_j)\n",
    "$$\n",
    "\n",
    "Further decompose the future observations:\n",
    "$$\n",
    "P(Y_{k+1:t} \\mid X_{k+1} = x_j)\n",
    "=\n",
    "P(Y_{k+1} \\mid X_{k+1} = x_j)\\,\n",
    "P(Y_{k+2:t} \\mid X_{k+1} = x_j)\n",
    "$$\n",
    "\n",
    "Recognizing the terms,\n",
    "$$\n",
    "P(Y_{k+1} \\mid X_{k+1} = x_j) = M_{j,y_{k+1}}, \\quad\n",
    "P(Y_{k+2:t} \\mid X_{k+1} = x_j) = \\beta_{k+1}(x_j)\n",
    "$$\n",
    "\n",
    "we obtain\n",
    "$$\n",
    "P(X_{k+1} = x_j, X_k = x_i, Y_{1:t})\n",
    "=\n",
    "\\alpha_k(x_i)\\,\n",
    "T_{ij}\\,\n",
    "M_{j,y_{k+1}}\\,\n",
    "\\beta_{k+1}(x_j)\n",
    "$$\n",
    "\n",
    "---\n",
    "\n",
    "### Step 3: Compute the denominator\n",
    "\n",
    "$$\n",
    "P(X_k = x_i, Y_{1:t})\n",
    "=\n",
    "P(Y_{1:k}, X_k = x_i)\\,\n",
    "P(Y_{k+1:t} \\mid X_k = x_i)\n",
    "$$\n",
    "\n",
    "Using the law of total probability over $X_{k+1}$,\n",
    "$$\n",
    "P(Y_{k+1:t} \\mid X_k = x_i)\n",
    "=\n",
    "\\sum_{j'}\n",
    "T_{ij'}\\,\n",
    "M_{j',y_{k+1}}\\,\n",
    "\\beta_{k+1}(x_{j'})\n",
    "$$\n",
    "\n",
    "Thus,\n",
    "$$\n",
    "P(X_k = x_i, Y_{1:t})\n",
    "=\n",
    "\\alpha_k(x_i)\n",
    "\\sum_{j'}\n",
    "T_{ij'}\\,\n",
    "M_{j',y_{k+1}}\\,\n",
    "\\beta_{k+1}(x_{j'})\n",
    "$$\n",
    "\n",
    "---\n",
    "\n",
    "### Step 4: Final expression\n",
    "\n",
    "Canceling $\\alpha_k(x_i)$ in numerator and denominator yields\n",
    "$$\n",
    "P(X_{k+1} = x_j \\mid X_k = x_i, Y_{1:t})\n",
    "=\n",
    "\\frac{\n",
    "T_{ij}\\,\n",
    "M_{j,y_{k+1}}\\,\n",
    "\\beta_{k+1}(x_j)\n",
    "}{\n",
    "\\sum_{j'}\n",
    "T_{ij'}\\,\n",
    "M_{j',y_{k+1}}\\,\n",
    "\\beta_{k+1}(x_{j'})\n",
    "}\n",
    "$$\n",
    "\n",
    "---\n",
    "\n",
    "## (2) Derive $P(X_k = x_i \\mid X_{k+1} = x_j, Y_{1:t})$\n",
    "\n",
    "By definition,\n",
    "$$\n",
    "P(X_k = x_i \\mid X_{k+1} = x_j, Y_{1:t})\n",
    "=\n",
    "\\frac{\n",
    "P(X_k = x_i, X_{k+1} = x_j, Y_{1:t})\n",
    "}{\n",
    "P(X_{k+1} = x_j, Y_{1:t})\n",
    "}\n",
    "$$\n",
    "\n",
    "From part (1),\n",
    "$$\n",
    "P(X_k = x_i, X_{k+1} = x_j, Y_{1:t})\n",
    "=\n",
    "\\alpha_k(x_i)\\,\n",
    "T_{ij}\\,\n",
    "M_{j,y_{k+1}}\\,\n",
    "\\beta_{k+1}(x_j)\n",
    "$$\n",
    "\n",
    "The denominator is obtained by marginalizing over $X_k$:\n",
    "$$\n",
    "P(X_{k+1} = x_j, Y_{1:t})\n",
    "=\n",
    "\\sum_{i'}\n",
    "\\alpha_k(x_{i'})\\,\n",
    "T_{i'j}\\,\n",
    "M_{j,y_{k+1}}\\,\n",
    "\\beta_{k+1}(x_j)\n",
    "$$\n",
    "\n",
    "Canceling common terms gives\n",
    "$$\n",
    "P(X_k = x_i \\mid X_{k+1} = x_j, Y_{1:t})\n",
    "=\n",
    "\\frac{\n",
    "\\alpha_k(x_i)\\,\n",
    "T_{ij}\n",
    "}{\n",
    "\\sum_{i'}\n",
    "\\alpha_k(x_{i'})\\,\n",
    "T_{i'j}\n",
    "}\n",
    "$$\n",
    "\n",
    "---\n",
    "\n",
    "## (3) Derive  \n",
    "$P(X_{k-1} = x_i, X_k = x_j, X_{k+1} = x_l \\mid Y_{1:t})$\n",
    "\n",
    "By definition,\n",
    "$$\n",
    "P(X_{k-1} = x_i, X_k = x_j, X_{k+1} = x_l \\mid Y_{1:t})\n",
    "=\n",
    "\\frac{\n",
    "P(X_{k-1} = x_i, X_k = x_j, X_{k+1} = x_l, Y_{1:t})\n",
    "}{\n",
    "P(Y_{1:t})\n",
    "}\n",
    "$$\n",
    "\n",
    "Split the observation sequence:\n",
    "$$\n",
    "Y_{1:t} = (Y_{1:k-1}, Y_k, Y_{k+1}, Y_{k+2:t})\n",
    "$$\n",
    "\n",
    "Using the HMM structure, the joint probability factorizes as\n",
    "$$\n",
    "\\alpha_{k-1}(x_i)\\,\n",
    "T_{ij}\\,\n",
    "M_{j,y_k}\\,\n",
    "T_{jl}\\,\n",
    "M_{l,y_{k+1}}\\,\n",
    "\\beta_{k+1}(x_l)\n",
    "$$\n",
    "\n",
    "Therefore,\n",
    "$$\n",
    "P(X_{k-1} = x_i, X_k = x_j, X_{k+1} = x_l \\mid Y_{1:t})\n",
    "=\n",
    "\\frac{\n",
    "\\alpha_{k-1}(x_i)\\,\n",
    "T_{ij}\\,\n",
    "M_{j,y_k}\\,\n",
    "T_{jl}\\,\n",
    "M_{l,y_{k+1}}\\,\n",
    "\\beta_{k+1}(x_l)\n",
    "}{\n",
    "\\sum_x \\alpha_t(x)\n",
    "}\n",
    "$$\n",
    "\n",
    "---\n",
    "\n",
    "## Summary of Results\n",
    "\n",
    "$$\n",
    "P(X_{k+1} = x_j \\mid X_k = x_i, Y_{1:t})\n",
    "=\n",
    "\\frac{\n",
    "T_{ij} M_{j,y_{k+1}} \\beta_{k+1}(x_j)\n",
    "}{\n",
    "\\sum_{j'} T_{ij'} M_{j',y_{k+1}} \\beta_{k+1}(x_{j'})\n",
    "}\n",
    "$$\n",
    "\n",
    "$$\n",
    "P(X_k = x_i \\mid X_{k+1} = x_j, Y_{1:t})\n",
    "=\n",
    "\\frac{\n",
    "\\alpha_k(x_i) T_{ij}\n",
    "}{\n",
    "\\sum_{i'} \\alpha_k(x_{i'}) T_{i'j}\n",
    "}\n",
    "$$\n",
    "\n",
    "$$\n",
    "P(X_{k-1} = x_i, X_k = x_j, X_{k+1} = x_l \\mid Y_{1:t})\n",
    "=\n",
    "\\frac{\n",
    "\\alpha_{k-1}(x_i) T_{ij} M_{j,y_k} T_{jl} M_{l,y_{k+1}} \\beta_{k+1}(x_l)\n",
    "}{\n",
    "\\sum_x \\alpha_t(x)\n",
    "}\n",
    "$$\n"
   ]
  }
 ],
 "metadata": {
  "language_info": {
   "name": "python"
  }
 },
 "nbformat": 4,
 "nbformat_minor": 5
}
